QR/PoK.ec
@@ -3,23 +3,22 @@ require import AllCore.
 require import Aux Permutation Basics List.
 
 require import SpecialSoundness.
-clone import PoK.
 
-clone import ComputationalPoK with op special_soundness_extract <- special_soundness_extract.
+
+
+clone import SpecialSoundnessTheory as SS with op special_soundness_extract <- special_soundness_extract.
+
 
 
 section.
-declare module P <: RewMaliciousProver {-HonestVerifier}.
+declare module P <: RewMaliciousProver {-HV}.
 
 declare axiom P_response_ll : islossless P.response.
 
 lemma qr_computational_PoK &m  s: 
   Pr[Extractor(P).extract(s) @ &m : IsSqRoot s res /\ unit s] >=
-   (Pr[Soundness(P, HonestVerifier).run(s) @ &m : res]^2
-     - (1%r/2%r) * Pr[Soundness(P, HonestVerifier).run(s) @ &m : res]).
-
-
-
+   (Pr[Soundness(P, HV).run(s) @ &m : res]^2
+     - (1%r/2%r) * Pr[Soundness(P, HV).run(s) @ &m : res]).
 apply (statistical_PoK P  _ &m s _ ).  apply P_response_ll. 
 smt (perfect_special_soundness).
 qed.
