QR/Soundness.ec
@@ -1,54 +1,33 @@
 pragma Goals:printall.
 require import AllCore DBool Bool List Distr RealExp.
-require import Basics Aux.
+require import Basics.
 
+require import PoK.
+import SS.
+
+clone import ExtractabilityTheory as ET.
 
 section.
 
-declare module P <: MaliciousProver {-HonestVerifier}.
+declare module P <: RewMaliciousProver {-HV}.
 declare axiom P_response_ll : islossless P.response.
-
-local lemma qr_soundness_ph s  :
-   ! in_language IsSqRoot s => 
-   phoare [ Soundness(P,HonestVerifier).run : arg = (s) ==> res ] <= (1%r/2%r).
-proof. move => qra.
-proc. inline*. 
-wp.
-seq 3 : ((statement) = (s) /\ statement0 = statement /\ commitment = commit) (1%r) (1%r/2%r) (0%r) (1%r).  auto. auto.
-exists* commit. elim*. move => cv.
-case (!IsQR cv).
-seq 1 : (!challenge0) (1%r/2%r) (0%r) (1%r/2%r) (1%r) (cv = commit /\ s = statement  /\ !IsQR cv).
-rnd.  skip. auto.
-hoare. call (_:true ==> true). auto.
-wp. auto. progress. rewrite H0. simplify.   timeout 20. smt. 
-rnd.  skip.  progress. 
-have -> : (fun (x : bool) => x) = pred1 true. smt. 
-have ->: mu1 (duniform [false; true]) true = 1%r/2%r. 
-rewrite duniform1E_uniq. auto. simplify. auto. auto.
-simplify. 
-conseq (_: _ ==> true). call (_: true ==> true). auto.  auto. auto.
-seq 1 : (!challenge0) (1%r/2%r) (0%r) (1%r/2%r) (1%r) (cv = commit /\ s = statement  /\ IsQR cv).
-rnd. skip. auto.
-hoare. 
-call (_:true ==> true). auto.  
-wp. skip. progress. rewrite H0. simplify. smt.
-rnd. skip. progress. 
-have -> : (fun (x : bool) => x) = pred1 true. smt. 
-have ->: mu1 (duniform [false; true]) true = 1%r/2%r. 
-rewrite duniform1E_uniq. auto. simplify. auto. auto.
-conseq (_: _ ==> true). call (_:true ==> true). auto.
-wp. skip. auto. auto.
-hoare.
-simplify. auto. call (_ : true ==> true).  auto. skip. auto. auto.
-qed.
 
 
 lemma qr_soundness &m s:
-    ! in_language IsSqRoot s =>
-     Pr[Soundness(P, HonestVerifier).run(s) @ &m : res]
+    ! in_language soundness_relation s =>
+     Pr[Soundness(P, HV).run(s) @ &m : res]
      <= 1%r/2%r.
-progress. byphoare (_: arg = (s) ==> _);auto.
-apply (qr_soundness_ph s);auto.
+progress.
+print computational_statistical_soundness.
+apply (computational_statistical_soundness Extractor HV P &m s
+ (fun (x:real) => x ^2 - 1%r/2%r * x) (1%r/2%r)   ).
+auto. simplify. 
+simplify.
+apply (qr_computational_PoK P _ &m s).
+apply P_response_ll.
+move => x. simplify.
+have -> : x ^ 2 = x * x. smt.
+smt.
 qed.
 
 
