QR/ZK.ec
@@ -1,13 +1,12 @@
 pragma Goals:printall.
 require import AllCore DBool Bool List Distr Int Aux DJoin.
 
-require import Permutation Basics Sim1Property.
-import Sim1Property.ZK.
+require import  Basics Sim1Property.
 
-import Sim1Property.QR_SZK.
+import OSS.
 import OMZK.
 
-clone import  StatisticalZKDeriv with op negl <- 0%r.
+clone import  StatisticalZK with op negl <- 0%r.
 
 
 require RewBasics.
@@ -15,12 +14,14 @@ clone import RewBasics as Rew with type sbits <- sbits.
 
 section.
 
-declare module V <: MaliciousVerifier{-HonestProver, -OMZK.MW.IFB.IM.W, -OMZK.MW.IFB.DW}.
+
+
+declare module V <: RewMaliciousVerifier{-HP, -OMZK.MW.IFB.IM.W, -OMZK.MW.IFB.DW}.
 declare module D <: ZKDistinguisher{-OMZK.MW.IFB.IM.W, -OMZK.MW.IFB.DW}.
 
 
-declare axiom Sim1_run_ll : forall (V0 <: MaliciousVerifier), islossless V0.challenge => islossless V0.summitup => islossless Sim1(V0).run.
-
+declare axiom Sim1_run_ll : forall (V0 <: RewMaliciousVerifier), islossless V0.challenge => islossless V0.summitup => islossless Sim1(V0).run.
+declare axiom D_guess_prop : equiv[ D.guess ~ D.guess : ={glob V, arg} ==> ={res} ].
 declare axiom V_summitup_ll : islossless V.summitup. 
 declare axiom V_challenge_ll : islossless V.challenge.
 declare axiom D_guess_ll : islossless D.guess.
@@ -40,12 +41,12 @@ declare axiom rewindable_V_plus :
 lemma qr_statistical_zk stat wit N &m:
         IsSqRoot stat  wit  => unit stat =>
         0 <= N =>
-        let real_prob = Pr[ZKReal(HonestProver, V, D).run(stat, wit) @ &m : res] in
+        let real_prob = Pr[ZKReal(HP, V, D).run(stat, wit) @ &m : res] in
         let ideal_prob = Pr[ZKIdeal(Simulator(Sim1), V, D).run(stat, wit, N) @ &m : res] in
           `|real_prob - ideal_prob| <= 2%r * (1%r / 2%r) ^ N.
 proof.
 progress.
-apply (statistical_zk HonestProver Sim1  V D _ _ _ _ _ _ _ stat wit  N
+apply (statistical_zk HP Sim1  V D _ _ _ _ _ _ _ _ stat wit  N
   (1%r/2%r) &m);auto. apply Sim1_run_ll. apply V_summitup_ll. apply V_challenge_ll. apply D_guess_ll.
 apply rewindable_V_plus. 
 
@@ -54,7 +55,7 @@ apply (sim1_rew_ph V).
 progress. 
 rewrite (sim1_prop V D _ _  _ _ _  p w  _ ).  apply (rewindable_A_plus V).
  exists f. split. auto. auto.
-auto. auto.   auto.  auto. auto.   auto. auto. 
+auto. auto.   auto.  auto. auto. apply D_guess_prop.
 rewrite (sim1assc V D _ _ _ _ &m stat  wit). apply (rewindable_A_plus V).
 apply rewindable_V_plus.
 apply V_summitup_ll.
