aux/WholeMsg.ec
@@ -1,0 +1,114 @@
+pragma Goals:printall.
+require import Distr DBool AllCore List.
+
+type message, ain.
+
+op m1, m2 : message.
+
+axiom m1_and_m2_diff : m1 <> m2.
+
+module type Tail = {
+  proc main(m : message, a : ain) : bool
+}.
+
+
+module W(T : Tail) = {
+  proc main(a : ain) = {
+    var m, r;
+    m <$ duniform [m1; m2];
+    r <@ T.main(m,a);
+    return r;
+  }
+}.
+
+
+section.
+
+
+declare module T <: Tail.
+
+local module W' = {
+  var m : message
+  proc main(a:ain) = {
+    var r;
+    m <$ duniform [m1; m2];
+    r <@ T.main(m,a);
+    return r;
+  }
+}.
+
+
+local lemma scx1 &m x:
+    Pr[ W'.main(x) @ &m : res /\ W'.m = m1 ]
+  = 1%r/2%r * Pr[ T.main(m1,x) @ &m : res ].
+proof. byphoare (_: (glob T) = (glob T){m} /\ a = x ==> _) => //. 
+proc. 
+pose z := (Pr[ T.main(m1,x) @ &m : res ]).
+seq 1 : (W'.m = m1) (1%r/2%r)  z (1%r/2%r) 0%r  ((glob T) = (glob T){m} /\ a = x).
+rnd.  skip. progress. 
+rnd.  skip. progress. rewrite duniformE =>//=. 
+have : m1 <> m2. apply m1_and_m2_diff. progress.
+case(m1 = m2) => //. progress. rewrite eq_sym in H0. rewrite H0. smt. 
+have phr : phoare[ T.main : (glob T) = (glob T){m} /\ arg = (m1, x) ==> res ] = Pr[ T.main(m1,x) @ &m : res ].
+bypr. progress. byequiv. 
+proc*. call (_:true). skip.
+progress. auto. smt. smt. auto. auto.
+call phr. skip. progress.
+hoare. call (_:true). skip. progress. rewrite H =>//=. 
+rewrite /z =>//.   
+qed.
+
+
+local lemma scx2 &m x:
+    Pr[ W'.main(x) @ &m : res /\ W'.m = m2 ]
+  = 1%r/2%r * Pr[ T.main(m2,x) @ &m : res ].
+proof. byphoare (_: (glob T) = (glob T){m} /\ a = x ==> _) =>//. 
+proc. 
+pose z := (Pr[ T.main(m2,x) @ &m : res ]).
+seq 1 : (W'.m = m2) (1%r/2%r)  z (1%r/2%r) 0%r  ((glob T) = (glob T){m} /\ a = x).
+rnd.  skip. auto. 
+rnd.  skip. progress. rewrite duniformE =>//=.  
+have : m1 <> m2. apply m1_and_m2_diff. progress.
+case(m1 = m2) => //. progress. rewrite H0. smt. 
+have phr : phoare[ T.main : (glob T) = (glob T){m} /\ arg = (m2, x) ==> res ] = Pr[ T.main(m2,x) @ &m : res ].
+bypr. progress. byequiv. 
+proc*. call (_:true). skip.
+progress. smt. smt. auto. auto.
+call phr. skip. progress.
+hoare. call (_:true). skip. progress. rewrite H =>//. 
+rewrite /z =>//.   
+qed.
+
+
+local lemma spc &m x :
+    Pr[ W'.main(x) @ &m : res ]
+   = Pr[ T.main(m1,x) @ &m : res ] / 2%r
+   + Pr[ T.main(m2,x)  @ &m : res ] / 2%r.
+proof. 
+have ->: Pr[ W'.main(x) @ &m : res ] =
+         Pr[ W'.main(x) @ &m : res /\ W'.m = m1 ] + Pr[ W'.main(x) @ &m : res /\ W'.m = m2 ].
+rewrite Pr[mu_split W'.m = m1]. 
+have ->: Pr[W'.main(x) @ &m : res /\ W'.m <> m1] = Pr[W'.main(x) @ &m : res /\ W'.m = m2]. 
+byequiv(_: _ ==> _) => //. proc. inline*.
+call(_:true). rnd. 
+skip. progress.  
+rewrite supp_duniform mem_seq2 in H. 
+elim H => [mL1 | mL2] => //.   
+have : m1 <> m2. apply m1_and_m2_diff. progress. rewrite eq_sym in H2. apply H2.
+reflexivity.
+rewrite scx1 scx2 =>//.  
+qed.
+
+   
+lemma splitcases &m x :
+    Pr[ W(T).main(x) @ &m : res ]
+   = Pr[ T.main(m1,x) @ &m : res ] / 2%r
+   + Pr[ T.main(m2,x)  @ &m : res ] / 2%r.
+proof.
+have  ->: Pr[ W(T).main(x) @ &m : res ] = Pr[ W'.main(x) @ &m : res ].
+byequiv. proc*. inline*. sim. auto. auto. 
+apply spc.
+qed.
+
+end section.
+    
